compiler/backend/semantics/dataSemScript.sml
@@ -1243,24 +1243,17 @@ Definition AppUnit_def:
   AppUnit =
     Seq
       (Seq
-        (Seq
-          (Assign 1 (IntOp (Const 0)) [] NONE)
-          (Seq
-            (Assign 2 (IntOp (Const 1)) [] NONE)
-            (Assign 3 (MemOp El) [0; 2] NONE)))
-        (Assign 4 (BlockOp Equal) [3; 1]
-           (SOME (list_to_num_set [3; 1; 0]))))
-      (If 4
+        (Assign 1 (BlockOp (ElemAt 1)) [0] NONE)
+        (Assign 2 (BlockOp (EqualConst (Int 0))) [1] NONE))
+      (If 2
         (Seq
           (Seq
-            (Assign 5 (BlockOp (Cons 0)) [] NONE)
-            (Seq
-              (Assign 6 (IntOp (Const 0)) [] NONE)
-              (Assign 7 (MemOp El) [0; 6] NONE)))
-          (Call NONE NONE [5; 0; 7] NONE))
+            (Assign 3 (BlockOp (Cons 0)) [] NONE)
+            (Assign 4 (BlockOp (ElemAt 0)) [0] NONE))
+          (Call NONE NONE [3; 0; 4] NONE))
         (Seq
-          (Assign 9 (BlockOp (Cons 0)) [] NONE)
-          (Call NONE (SOME bvl_num_stubs) [9; 0] NONE)))
+          (Assign 6 (BlockOp (Cons 0)) [] NONE)
+          (Call NONE (SOME bvl_num_stubs) [6; 0] NONE)))
 End
 
 Definition evaluate_def:
